test-mutable-compile.sh
@@ -1,0 +1,1 @@
+g++ lib/DataStructures/lib/DataStructures/MutableBtree.i.cpp -o MutableBtreeTest -I .dafny/dafny/Binaries/ -I lib/DataStructures/ -std=c++17
